systems/FailureRecorderDynamic.v
@@ -340,7 +340,7 @@ Variable onet : ordered_dynamic_network.
 
 Variable failed : list name.
 
-Variable tr : list (name * (input + list output)).
+Variable tr : list (name * (input + output)).
 
 Hypothesis H_step : step_o_d_f_star step_o_d_f_init (failed, onet) tr.
 
@@ -426,7 +426,7 @@ Variable onet : ordered_dynamic_network.
 
 Variable failed : list name.
 
-Variable tr : list (name * (input + list output)).
+Variable tr : list (name * (input + output)).
 
 Hypothesis H_step : step_o_d_f_star step_o_d_f_init (failed, onet) tr.
 
@@ -665,7 +665,7 @@ Variable onet : ordered_dynamic_network.
 
 Variable failed : list name.
 
-Variable tr : list (name * (input + list output)).
+Variable tr : list (name * (input + output)).
 
 Hypothesis H_step : step_o_d_f_star step_o_d_f_init (failed, onet) tr.
 
@@ -1305,7 +1305,7 @@ Variable onet : ordered_dynamic_network.
 
 Variable failed : list name.
 
-Variable tr : list (name * (input + list output)).
+Variable tr : list (name * (input + output)).
 
 Hypothesis H_step : step_o_d_f_star step_o_d_f_init (failed, onet) tr.
 
